Rename a few things in the Coq development to hopefully make the use of Simplicity algebras a bit less confusing.

Coq/Simplicity/Alg.v
@@ -20,48 +20,48 @@ Record class (term : Ty -> Ty -> Type) := Class
 }.
 End Class.
 
-Structure type := Pack { carrier :> Ty -> Ty -> Type; class_of :> Class.class carrier }.
+Structure Algebra := Pack { domain :> Ty -> Ty -> Type; class_of :> Class.class domain }.
 
-Record ReynoldsRel (term1 term2 : type) :=
- { rel :> forall {A B}, term1 A B -> term2 A B -> Prop
- ; _ : forall A, rel (Class.iden term1) (@Class.iden _ term2 A)
- ; _ : forall A B C s1 s2 t1 t2, rel s1 s2 -> rel t1 t2 -> rel (Class.comp term1 s1 t1) (@Class.comp _ term2 A B C s2 t2)
- ; _ : forall A, rel (Class.unit term1) (@Class.unit _ term2 A)
- ; _ : forall A B C t1 t2, rel t1 t2 -> rel (Class.injl term1 t1) (@Class.injl _ term2 A B C t2)
- ; _ : forall A B C t1 t2, rel t1 t2 -> rel (Class.injr term1 t1) (@Class.injr _ term2 A B C t2)
- ; _ : forall A B C D s1 s2 t1 t2, rel s1 s2 -> rel t1 t2 -> rel (Class.case term1 s1 t1) (@Class.case _ term2 A B C D s2 t2)
- ; _ : forall A B C s1 s2 t1 t2, rel s1 s2 -> rel t1 t2 -> rel (Class.pair term1 s1 t1) (@Class.pair _ term2 A B C s2 t2)
- ; _ : forall A B C t1 t2, rel t1 t2 -> rel (Class.take term1 t1) (@Class.take _ term2 A B C t2)
- ; _ : forall A B C t1 t2, rel t1 t2 -> rel (Class.drop term1 t1) (@Class.drop _ term2 A B C t2)
+Record ReynoldsRel (alg1 alg2 : Algebra) :=
+ { rel :> forall {A B}, alg1 A B -> alg2 A B -> Prop
+ ; _ : forall A, rel (Class.iden alg1) (@Class.iden _ alg2 A)
+ ; _ : forall A B C s1 s2 t1 t2, rel s1 s2 -> rel t1 t2 -> rel (Class.comp alg1 s1 t1) (@Class.comp _ alg2 A B C s2 t2)
+ ; _ : forall A, rel (Class.unit alg1) (@Class.unit _ alg2 A)
+ ; _ : forall A B C t1 t2, rel t1 t2 -> rel (Class.injl alg1 t1) (@Class.injl _ alg2 A B C t2)
+ ; _ : forall A B C t1 t2, rel t1 t2 -> rel (Class.injr alg1 t1) (@Class.injr _ alg2 A B C t2)
+ ; _ : forall A B C D s1 s2 t1 t2, rel s1 s2 -> rel t1 t2 -> rel (Class.case alg1 s1 t1) (@Class.case _ alg2 A B C D s2 t2)
+ ; _ : forall A B C s1 s2 t1 t2, rel s1 s2 -> rel t1 t2 -> rel (Class.pair alg1 s1 t1) (@Class.pair _ alg2 A B C s2 t2)
+ ; _ : forall A B C t1 t2, rel t1 t2 -> rel (Class.take alg1 t1) (@Class.take _ alg2 A B C t2)
+ ; _ : forall A B C t1 t2, rel t1 t2 -> rel (Class.drop alg1 t1) (@Class.drop _ alg2 A B C t2)
  }.
 
-Definition Reynolds {A B} (x y : forall (term : type), term A B) : Prop :=
-  forall (term1 term2 : type) (R : ReynoldsRel term1 term2), R A B (x term1) (y term2).
+Definition Reynolds {A B} (x y : forall (alg : Algebra), alg A B) : Prop :=
+  forall alg1 alg2 (R : ReynoldsRel alg1 alg2), R A B (x alg1) (y alg2).
 
-Definition Parametric {A B} (x : forall (term : type), term A B) : Prop := Reynolds x x.
+Definition Parametric {A B} (x : forall (alg : Algebra), alg A B) : Prop := Reynolds x x.
 
 Section Term.
 
-Fixpoint eval {A B} (x : Simplicity.Core.Term A B) {term : type} : term A B :=
-match x in Simplicity.Core.Term A B return term A B with
-| Simplicity.Core.iden => Class.iden term
-| Simplicity.Core.comp s t => Class.comp term (eval s) (eval t)
-| Simplicity.Core.unit => Class.unit term
-| Simplicity.Core.injl t => Class.injl term (eval t)
-| Simplicity.Core.injr t => Class.injr term (eval t)
-| Simplicity.Core.case s t => Class.case term (eval s) (eval t)
-| Simplicity.Core.pair s t => Class.pair term (eval s) (eval t)
-| Simplicity.Core.take t => Class.take term (eval t)
-| Simplicity.Core.drop t => Class.drop term (eval t)
+Fixpoint eval {A B} (x : Simplicity.Core.Term A B) {alg : Algebra} : alg A B :=
+match x in Simplicity.Core.Term A B return alg A B with
+| Simplicity.Core.iden => Class.iden alg
+| Simplicity.Core.comp s t => Class.comp alg (eval s) (eval t)
+| Simplicity.Core.unit => Class.unit alg
+| Simplicity.Core.injl t => Class.injl alg (eval t)
+| Simplicity.Core.injr t => Class.injr alg (eval t)
+| Simplicity.Core.case s t => Class.case alg (eval s) (eval t)
+| Simplicity.Core.pair s t => Class.pair alg (eval s) (eval t)
+| Simplicity.Core.take t => Class.take alg (eval t)
+| Simplicity.Core.drop t => Class.drop alg (eval t)
 end.
 
 Lemma eval_Parametric {A B} (x : Simplicity.Core.Term A B) : Parametric (@eval A B x).
 Proof.
-intros term1 term2 [R].
+intros alg1 alg2 [R].
 induction x; simpl; auto.
 Qed.
 
-Canonical Structure Term : type := Pack (Class.Class
+Canonical Structure Term : Algebra := Pack (Class.Class
   Simplicity.Core.Term
   (@Simplicity.Core.iden)
   (@Simplicity.Core.comp)
@@ -79,10 +79,10 @@ Proof.
 induction x; simpl; congruence.
 Qed.
 
-Lemma term_eval {A B} (x : forall (term : type), term A B) (Hx : Parametric x) (term : type) :
-  x term = eval (x Term).
+Lemma term_eval {A B} (x : forall alg : Algebra, alg A B) (Hx : Parametric x) (alg : Algebra) :
+  x alg = eval (x Term).
 Proof.
-refine (Hx _ _ (Build_ReynoldsRel Term term (fun a b x y => y = eval x) _ _ _ _ _ _ _ _ _));
+refine (Hx _ _ (Build_ReynoldsRel Term alg (fun a b x y => y = eval x) _ _ _ _ _ _ _ _ _));
 intros; simpl; congruence.
 Qed.
 
@@ -91,21 +91,21 @@ End Term.
 End Core.
 
 Coercion Core.rel : Core.ReynoldsRel >-> Funclass.
-Coercion Core.carrier : Core.type >-> Funclass.
+Coercion Core.domain : Core.Algebra >-> Funclass.
 
 Section Core_Combinators.
 
-Definition iden {A} {term : Core.type} : term A A := Core.Class.iden (Core.class_of term).
-Definition comp {A B C} {term : Core.type} : term A B -> term B C -> term A C := Core.Class.comp (Core.class_of term).
-Definition unit {A} {term : Core.type} : term A Unit := Core.Class.unit (Core.class_of term).
-Definition injl {A B C} {term : Core.type} : term A B -> term A (B + C) := Core.Class.injl (Core.class_of term).
-Definition injr {A B C} {term : Core.type} : term A C -> term A (B + C) := Core.Class.injr (Core.class_of term).
-Definition case {A B C D} {term : Core.type} : term (A * C) D -> term (B * C) D -> term ((A + B) * C) D := Core.Class.case (Core.class_of term).
-Definition pair {A B C} {term : Core.type} : term A B -> term A C -> term A (B * C) := Core.Class.pair (Core.class_of term).
-Definition take {A B C} {term : Core.type} : term A C -> term (A * B) C := Core.Class.take (Core.class_of term).
-Definition drop {A B C} {term : Core.type} : term B C -> term (A * B) C := Core.Class.drop (Core.class_of term).
+Definition iden {A} {alg : Core.Algebra} : alg A A := Core.Class.iden (Core.class_of alg).
+Definition comp {A B C} {alg : Core.Algebra} : alg A B -> alg B C -> alg A C := Core.Class.comp (Core.class_of alg).
+Definition unit {A} {alg : Core.Algebra} : alg A Unit := Core.Class.unit (Core.class_of alg).
+Definition injl {A B C} {alg : Core.Algebra} : alg A B -> alg A (B + C) := Core.Class.injl (Core.class_of alg).
+Definition injr {A B C} {alg : Core.Algebra} : alg A C -> alg A (B + C) := Core.Class.injr (Core.class_of alg).
+Definition case {A B C D} {alg : Core.Algebra} : alg (A * C) D -> alg (B * C) D -> alg ((A + B) * C) D := Core.Class.case (Core.class_of alg).
+Definition pair {A B C} {alg : Core.Algebra} : alg A B -> alg A C -> alg A (B * C) := Core.Class.pair (Core.class_of alg).
+Definition take {A B C} {alg : Core.Algebra} : alg A C -> alg (A * B) C := Core.Class.take (Core.class_of alg).
+Definition drop {A B C} {alg : Core.Algebra} : alg B C -> alg (A * B) C := Core.Class.drop (Core.class_of alg).
 
-Lemma iden_Parametric {term1 term2 : Core.type} (R : Core.ReynoldsRel term1 term2)
+Lemma iden_Parametric {alg1 alg2 : Core.Algebra} (R : Core.ReynoldsRel alg1 alg2)
   {A} : R A A iden iden.
 Proof.
 unfold iden.
@@ -113,7 +113,7 @@ destruct R as [R].
 simpl; auto.
 Qed.
 
-Lemma comp_Parametric {term1 term2 : Core.type} (R : Core.ReynoldsRel term1 term2)
+Lemma comp_Parametric {alg1 alg2 : Core.Algebra} (R : Core.ReynoldsRel alg1 alg2)
   {A B C} s1 s2 t1 t2 : R A B s1 s2 -> R B C t1 t2 -> R A C (comp s1 t1) (comp s2 t2).
 Proof.
 unfold comp.
@@ -121,7 +121,7 @@ destruct R as [R].
 simpl; auto.
 Qed.
 
-Lemma unit_Parametric {term1 term2 : Core.type} (R : Core.ReynoldsRel term1 term2)
+Lemma unit_Parametric {alg1 alg2 : Core.Algebra} (R : Core.ReynoldsRel alg1 alg2)
   {A} : R A Unit unit unit.
 Proof.
 unfold unit.
@@ -129,7 +129,7 @@ destruct R as [R].
 simpl; auto.
 Qed.
 
-Lemma injl_Parametric {term1 term2 : Core.type} (R : Core.ReynoldsRel term1 term2)
+Lemma injl_Parametric {alg1 alg2 : Core.Algebra} (R : Core.ReynoldsRel alg1 alg2)
   {A B C} t1 t2 : R A B t1 t2 -> R A (B + C) (injl t1) (injl t2).
 Proof.
 unfold injl.
@@ -137,7 +137,7 @@ destruct R as [R].
 simpl; auto.
 Qed.
 
-Lemma injr_Parametric {term1 term2 : Core.type} (R : Core.ReynoldsRel term1 term2)
+Lemma injr_Parametric {alg1 alg2 : Core.Algebra} (R : Core.ReynoldsRel alg1 alg2)
   {A B C} t1 t2 : R A C t1 t2 -> R A (B + C) (injr t1) (injr t2).
 Proof.
 unfold injr.
@@ -145,7 +145,7 @@ destruct R as [R].
 simpl; auto.
 Qed.
 
-Lemma case_Parametric {term1 term2 : Core.type} (R : Core.ReynoldsRel term1 term2)
+Lemma case_Parametric {alg1 alg2 : Core.Algebra} (R : Core.ReynoldsRel alg1 alg2)
   {A B C D} s1 s2 t1 t2 : R (A * C) D s1 s2 -> R (B * C) D t1 t2 -> R ((A + B) * C) D (case s1 t1) (case s2 t2).
 Proof.
 unfold case.
@@ -153,7 +153,7 @@ destruct R as [R].
 simpl; auto.
 Qed.
 
-Lemma pair_Parametric {term1 term2 : Core.type} (R : Core.ReynoldsRel term1 term2)
+Lemma pair_Parametric {alg1 alg2 : Core.Algebra} (R : Core.ReynoldsRel alg1 alg2)
   {A B C} s1 s2 t1 t2 : R A B s1 s2 -> R A C t1 t2 -> R A (B * C) (pair s1 t1) (pair s2 t2).
 Proof.
 unfold pair.
@@ -161,7 +161,7 @@ destruct R as [R].
 simpl; auto.
 Qed.
 
-Lemma take_Parametric {term1 term2 : Core.type} (R : Core.ReynoldsRel term1 term2)
+Lemma take_Parametric {alg1 alg2 : Core.Algebra} (R : Core.ReynoldsRel alg1 alg2)
   {A B C} t1 t2 : R A C t1 t2 -> R (A * B) C (take t1) (take t2).
 Proof.
 unfold take.
@@ -169,7 +169,7 @@ destruct R as [R].
 simpl; auto.
 Qed.
 
-Lemma drop_Parametric {term1 term2 : Core.type} (R : Core.ReynoldsRel term1 term2)
+Lemma drop_Parametric {alg1 alg2 : Core.Algebra} (R : Core.ReynoldsRel alg1 alg2)
   {A B C} t1 t2 : R B C t1 t2 -> R (A * B) C (drop t1) (drop t2).
 Proof.
 unfold drop.
@@ -199,7 +199,7 @@ Notation "'I' x" := (drop x) (at level 0, right associativity) : term_scope.
 
 Section CoreSem.
 
-Definition CoreSem : Core.type := Core.Pack (Core.Class.Class (fun A B => A -> B)
+Definition CoreSem : Core.Algebra := Core.Pack (Core.Class.Class (fun A B => A -> B)
   (fun A a => a)
   (fun A B C s t a => t (s a))
   (fun A _ => tt)
@@ -215,11 +215,11 @@ Definition CoreSem : Core.type := Core.Pack (Core.Class.Class (fun A B => A -> B
   (fun A B C t ab => t (snd ab))
 ).
 
-Lemma CoreSem_correct {A B} (x : Simplicity.Core.Term A B) : Simplicity.Core.eval x = Core.eval x (term := CoreSem).
+Lemma CoreSem_correct {A B} (x : Simplicity.Core.Term A B) : Simplicity.Core.eval x = Core.eval x (alg := CoreSem).
 Proof.
 induction x; simpl; try first [rewrite IHx | rewrite IHx1, IHx2]; reflexivity.
 Qed.
 
 End CoreSem.
 
-Notation "|[ x ]|" := (x : Core.carrier CoreSem _ _) : core_alg_scope.
+Notation "|[ x ]|" := (x : Core.domain CoreSem _ _) : core_alg_scope.
