Coq/Simplicity/Arith.v
@@ -188,45 +188,45 @@ Qed.
 
 Section Definitions.
 
-Definition adderBit {term : Core.type} : term (Bit * Bit) (Bit * Bit) :=
+Definition adderBit {term : Core.Algebra} : term (Bit * Bit) (Bit * Bit) :=
   cond (iden &&& not iden) (false &&& iden).
 
-Definition fullAdderBit {term : Core.type} : term ((Bit * Bit) * Bit) (Bit * Bit) :=
+Definition fullAdderBit {term : Core.Algebra} : term ((Bit * Bit) * Bit) (Bit * Bit) :=
   let add := adderBit in
     take add &&& I H
 >>> O O H &&& (O I H &&& I H >>> add)
 >>> cond true O H &&& I I H.
 
-Definition buildFullAdder {W} {term : Core.type} (rec : term ((W * W) * Bit) (Bit * W)) :
+Definition buildFullAdder {W} {term : Core.Algebra} (rec : term ((W * W) * Bit) (Bit * W)) :
   term (((W * W) * (W * W)) * Bit) (Bit * (W * W)) :=
     take (O O H &&& I O H) &&& (take (O I H &&& I I H) &&& I H >>> rec)
 >>> I I H &&& (O H &&& I O H >>> rec)
 >>> I O H &&& (I I H &&& O H).
 
-Fixpoint fullAdder {n : nat} {term : Core.type} : term ((Word n * Word n) * Bit) (Bit * Word n) :=
+Fixpoint fullAdder {n : nat} {term : Core.Algebra} : term ((Word n * Word n) * Bit) (Bit * Word n) :=
 match n with
 | 0 => fullAdderBit
 | S n => buildFullAdder fullAdder
 end.
 
-Definition buildAdder {W} {term : Core.type} (fa : term ((W * W) * Bit) (Bit * W)) (rec : term (W * W) (Bit * W)) :
+Definition buildAdder {W} {term : Core.Algebra} (fa : term ((W * W) * Bit) (Bit * W)) (rec : term (W * W) (Bit * W)) :
   term ((W * W) * (W * W)) (Bit * (W * W)) :=
     (O O H &&& I O H)
 &&& (O I H &&& I I H >>> rec)
 >>> I I H &&& (O H &&& I O H >>> fa)
 >>> I O H &&& (I I H &&& O H).
 
-Fixpoint adder {n : nat} {term : Core.type} : term (Word n * Word n) (Bit * Word n) :=
+Fixpoint adder {n : nat} {term : Core.Algebra} : term (Word n * Word n) (Bit * Word n) :=
 match n with
 | 0 => adderBit
 | S n => buildAdder fullAdder adder
 end.
 
-Definition fullMultiplierBit {term : Core.type} : term ((Bit * Bit) * (Bit * Bit)) (Word 1) :=
+Definition fullMultiplierBit {term : Core.Algebra} : term ((Bit * Bit) * (Bit * Bit)) (Word 1) :=
     drop iden &&& take (cond iden false)
 >>> fullAdderBit.
 
-Definition buildFullMultiplier {W} {term : Core.type} (rec : term ((W * W) * (W * W)) (W * W)) :
+Definition buildFullMultiplier {W} {term : Core.Algebra} (rec : term ((W * W) * (W * W)) (W * W)) :
   term (((W * W) * (W * W)) * ((W * W) * (W * W))) (((W * W) * (W * W))) :=
     take (O O H &&& (I O H &&& O I H))
 &&& ((take (O O H &&& I I H) &&& drop (O O H &&& I O H) >>> rec)
@@ -235,16 +235,16 @@ Definition buildFullMultiplier {W} {term : Core.type} (rec : term ((W * W) * (W 
 &&& (drop (O O H &&& I I H) &&& (O I H &&& drop (O I H &&& I O H) >>> rec))
 >>> (O H &&& drop (I O H &&& O O H) >>> rec) &&& drop (I I H &&& O I H).
 
-Fixpoint fullMultiplier {n : nat} {term : Core.type} : term ((Word n * Word n) * (Word n * Word n)) (Word (S n)) :=
+Fixpoint fullMultiplier {n : nat} {term : Core.Algebra} : term ((Word n * Word n) * (Word n * Word n)) (Word (S n)) :=
 match n with
 | 0 => fullMultiplierBit
 | S n => buildFullMultiplier fullMultiplier
 end.
 
-Definition multiplierBit {term : Core.type} : term (Bit * Bit) (Word 1) :=
+Definition multiplierBit {term : Core.Algebra} : term (Bit * Bit) (Word 1) :=
     false &&& cond iden false.
 
-Definition buildMultiplier {W} {term : Core.type} (fm : term ((W * W) * (W * W)) (W * W)) (rec : term (W * W) (W * W)) :
+Definition buildMultiplier {W} {term : Core.Algebra} (fm : term ((W * W) * (W * W)) (W * W)) (rec : term (W * W) (W * W)) :
   term ((W * W) * (W * W)) ((W * W) * (W * W)) :=
     (O O H &&& (I O H &&& O I H))
 &&& ((O O H &&& I I H >>> rec) &&& (O I H &&& I I H >>> rec))
@@ -252,7 +252,7 @@ Definition buildMultiplier {W} {term : Core.type} (fm : term ((W * W) * (W * W))
 &&& (drop (O O H &&& I I H) &&& (O I H &&& drop (O I H &&& I O H) >>> fm))
 >>> (O H &&& drop (I O H &&& O O H) >>> fm) &&& drop (I I H &&& O I H).
 
-Fixpoint multiplier {n : nat} {term : Core.type} : term (Word n * Word n) (Word (S n)) :=
+Fixpoint multiplier {n : nat} {term : Core.Algebra} : term (Word n * Word n) (Word (S n)) :=
 match n with
 | 0 => multiplierBit
 | S n => buildMultiplier fullMultiplier multiplier
@@ -377,21 +377,21 @@ rewrite two_power_nat_correct, Zpower_nat_is_exp, <- two_power_nat_correct; fold
 set (X := toZ _); ring.
 Qed.
 
-Lemma adderBit_Parametric {term1 term2 : Core.type} (R : Core.ReynoldsRel term1 term2) : R _ _ adderBit adderBit.
+Lemma adderBit_Parametric {term1 term2 : Core.Algebra} (R : Core.ReynoldsRel term1 term2) : R _ _ adderBit adderBit.
 Proof.
 unfold adderBit.
 auto with parametricity.
 Qed.
 Hint Resolve adderBit_Parametric : parametricity.
 
-Lemma fullAdderBit_Parametric {term1 term2 : Core.type} (R : Core.ReynoldsRel term1 term2) : R _ _ fullAdderBit fullAdderBit.
+Lemma fullAdderBit_Parametric {term1 term2 : Core.Algebra} (R : Core.ReynoldsRel term1 term2) : R _ _ fullAdderBit fullAdderBit.
 Proof.
 unfold fullAdderBit.
 auto 10 with parametricity.
 Qed.
 Hint Resolve fullAdderBit_Parametric : parametricity.
 
-Lemma buildFullAdder_Parametric {term1 term2 : Core.type} (R : Core.ReynoldsRel term1 term2)
+Lemma buildFullAdder_Parametric {term1 term2 : Core.Algebra} (R : Core.ReynoldsRel term1 term2)
   {W} t1 t2 : R _ (Bit * W) t1 t2 -> R _ _ (buildFullAdder t1) (buildFullAdder t2).
 Proof.
 unfold buildFullAdder.
@@ -399,14 +399,14 @@ auto 10 with parametricity.
 Qed.
 Hint Resolve buildFullAdder_Parametric : parametricity.
 
-Lemma fullAdder_Parametric {term1 term2 : Core.type} (R : Core.ReynoldsRel term1 term2)
+Lemma fullAdder_Parametric {term1 term2 : Core.Algebra} (R : Core.ReynoldsRel term1 term2)
   {n} : R _ _ fullAdder (@fullAdder n _).
 Proof.
 induction n; simpl; auto with parametricity.
 Qed.
 Hint Resolve fullAdder_Parametric : parametricity.
 
-Lemma buildAdder_Parametric {term1 term2 : Core.type} (R : Core.ReynoldsRel term1 term2)
+Lemma buildAdder_Parametric {term1 term2 : Core.Algebra} (R : Core.ReynoldsRel term1 term2)
   {W} s1 s2 t1 t2 : R _ (Bit * W) s1 s2 -> R _ (Bit * W) t1 t2 -> R _ _ (buildAdder s1 t1) (buildAdder s2 t2).
 Proof.
 unfold buildAdder.
@@ -414,21 +414,21 @@ auto 10 with parametricity.
 Qed.
 Hint Resolve buildAdder_Parametric : parametricity.
 
-Lemma adder_Parametric {term1 term2 : Core.type} (R : Core.ReynoldsRel term1 term2)
+Lemma adder_Parametric {term1 term2 : Core.Algebra} (R : Core.ReynoldsRel term1 term2)
   {n} : R _ _ adder (@adder n _).
 Proof.
 induction n; simpl; auto with parametricity.
 Qed.
 Hint Resolve adder_Parametric : parametricity.
 
-Lemma fullMultiplierBit_Parametric {term1 term2 : Core.type} (R : Core.ReynoldsRel term1 term2) : R _ _ fullMultiplierBit fullMultiplierBit.
+Lemma fullMultiplierBit_Parametric {term1 term2 : Core.Algebra} (R : Core.ReynoldsRel term1 term2) : R _ _ fullMultiplierBit fullMultiplierBit.
 Proof.
 unfold fullMultiplierBit.
 auto with parametricity.
 Qed.
 Hint Resolve fullMultiplierBit_Parametric : parametricity.
 
-Lemma buildFullMultiplier_Parametric {term1 term2 : Core.type} (R : Core.ReynoldsRel term1 term2)
+Lemma buildFullMultiplier_Parametric {term1 term2 : Core.Algebra} (R : Core.ReynoldsRel term1 term2)
   {W} t1 t2 : R _ (W * W) t1 t2 -> R _ _ (buildFullMultiplier t1) (buildFullMultiplier t2).
 Proof.
 unfold buildFullMultiplier.
@@ -436,14 +436,14 @@ auto 15 with parametricity.
 Qed.
 Hint Resolve buildFullMultiplier_Parametric : parametricity.
 
-Lemma fullMultiplier_Parametric {term1 term2 : Core.type} (R : Core.ReynoldsRel term1 term2)
+Lemma fullMultiplier_Parametric {term1 term2 : Core.Algebra} (R : Core.ReynoldsRel term1 term2)
   {n} : R _ (Word n * Word n) fullMultiplier (@fullMultiplier n _).
 Proof.
 induction n; simpl; auto with parametricity.
 Qed.
 Hint Resolve fullMultiplier_Parametric : parametricity.
 
-Lemma multiplierBit_Parametric {term1 term2 : Core.type} (R : Core.ReynoldsRel term1 term2) : R _ _ multiplierBit multiplierBit.
+Lemma multiplierBit_Parametric {term1 term2 : Core.Algebra} (R : Core.ReynoldsRel term1 term2) : R _ _ multiplierBit multiplierBit.
 Proof.
 simpl.
 unfold multiplierBit.
@@ -451,7 +451,7 @@ auto with parametricity.
 Qed.
 Hint Resolve multiplierBit_Parametric : parametricity.
 
-Lemma buildMultiplier_Parametric {term1 term2 : Core.type} (R : Core.ReynoldsRel term1 term2)
+Lemma buildMultiplier_Parametric {term1 term2 : Core.Algebra} (R : Core.ReynoldsRel term1 term2)
   {W} s1 s2 t1 t2 : R _ (W * W) s1 s2 -> R _ (W * W) t1 t2 -> R _ _ (buildMultiplier s1 t1) (buildMultiplier s2 t2).
 Proof.
 unfold buildMultiplier.
@@ -459,7 +459,7 @@ auto 15 with parametricity.
 Qed.
 Hint Resolve buildMultiplier_Parametric : parametricity.
 
-Lemma multiplier_Parametric {term1 term2 : Core.type} (R : Core.ReynoldsRel term1 term2)
+Lemma multiplier_Parametric {term1 term2 : Core.Algebra} (R : Core.ReynoldsRel term1 term2)
   {n} : R _ _ multiplier (@multiplier n _).
 Proof.
 induction n; simpl; auto 20 with parametricity.
