Coq/Simplicity/Bit.v
@@ -10,18 +10,18 @@ Notation "'Bit.one'" := (inr tt).
 
 Section Definitions.
 
-Definition false {A} {term : Core.type} : term A Bit := injl unit.
-Definition true {A} {term : Core.type} : term A Bit := injr unit.
+Definition false {A} {term : Core.Algebra} : term A Bit := injl unit.
+Definition true {A} {term : Core.Algebra} : term A Bit := injr unit.
 
-Definition cond {A B} {term : Core.type} (thn els : term A B) : term (Bit * A) B :=
+Definition cond {A B} {term : Core.Algebra} (thn els : term A B) : term (Bit * A) B :=
   case (drop els) (drop thn).
 
-Definition not {A} {term : Core.type} (t : term A Bit) : term A Bit :=
+Definition not {A} {term : Core.Algebra} (t : term A Bit) : term A Bit :=
   t &&& unit >>> cond false true.
 
 End Definitions.
 
-Lemma false_Parametric {term1 term2 : Core.type} (R : Core.ReynoldsRel term1 term2)
+Lemma false_Parametric {term1 term2 : Core.Algebra} (R : Core.ReynoldsRel term1 term2)
   {A} : R A Bit false false.
 Proof.
 unfold false.
@@ -29,7 +29,7 @@ auto with parametricity.
 Qed.
 Hint Immediate false_Parametric : parametricity.
 
-Lemma true_Parametric {term1 term2 : Core.type} (R : Core.ReynoldsRel term1 term2)
+Lemma true_Parametric {term1 term2 : Core.Algebra} (R : Core.ReynoldsRel term1 term2)
   {A} : R A Bit true true.
 Proof.
 unfold true.
@@ -37,7 +37,7 @@ auto with parametricity.
 Qed.
 Hint Immediate true_Parametric : parametricity.
 
-Lemma cond_Parametric {term1 term2 : Core.type} (R : Core.ReynoldsRel term1 term2)
+Lemma cond_Parametric {term1 term2 : Core.Algebra} (R : Core.ReynoldsRel term1 term2)
   {A B} s1 s2 t1 t2 : R A B s1 s2 -> R A B t1 t2 -> R (Bit * A) B (cond s1 t1) (cond s2 t2).
 Proof.
 unfold cond.
@@ -45,7 +45,7 @@ auto with parametricity.
 Qed.
 Hint Resolve cond_Parametric : parametricity.
 
-Lemma not_Parametric {term1 term2 : Core.type} (R : Core.ReynoldsRel term1 term2)
+Lemma not_Parametric {term1 term2 : Core.Algebra} (R : Core.ReynoldsRel term1 term2)
   {A} t1 t2 : R A Bit t1 t2 -> R A Bit (not t1) (not t2).
 Proof.
 unfold not.
